src/cbor/spec/raw/CBOR.Spec.API.Format.fst
@@ -35,3 +35,15 @@ let cbor_det_parse_prefix x =
 
 let cbor_det_serialize_parse x =
   RF.serialize_parse_cbor (R.mk_det_raw_cbor x)
+
+let cbor_det_serialize_tag tag =
+  RF.serialize_cbor_tag (RF.mk_raw_uint64 tag)
+
+let cbor_det_serialize_tag_length tag =
+  RF.serialize_cbor_tag_length (RF.mk_raw_uint64 tag)
+
+let cbor_det_serialize_tag_correct tag payload =
+  R.mk_cbor_eq (R.Tagged (RF.mk_raw_uint64 tag) (R.mk_det_raw_cbor payload));
+  R.mk_det_raw_cbor_mk_cbor (R.Tagged (RF.mk_raw_uint64 tag) (R.mk_det_raw_cbor payload));
+  assert (R.mk_det_raw_cbor (pack (CTagged tag payload)) == R.Tagged (RF.mk_raw_uint64 tag) (R.mk_det_raw_cbor payload));
+  RF.serialize_cbor_tag_correct (RF.mk_raw_uint64 tag) (R.mk_det_raw_cbor payload)
